src/x86/listimp.v
@@ -20,7 +20,7 @@ Definition inlineTail (r1 r2:GPReg64) :program :=
 
 (* Head is in r1, tail is in r2, result in EDI, ESI trashed *)
 Definition updateCons (r1 r2:GPReg64) :program :=
-    SUB RDI, (BOPArgI OpSize8 (16:DWORD));;
+    SUB RDI, (#16 : IMM _);;
     MOV QWORD PTR [RDI], r1;;
     MOV QWORD PTR [RDI+8], r2.
 
