src/x86/win/messagebox.v
@@ -12,13 +12,19 @@ Import Prenex Implicits.
 Open Scope string_scope.
 Open Scope instr_scope.
 
+Require Import addr.
 (*=messageBoxProg *)
 Definition mbProg: topprog :=
   IMPORTDLL "user32.dll";
   IMPORT "MessageBoxA" as MessageBoxA;
   GLOBAL message; GLOBAL title;
 SECTION CODE
-  call_with stdcall 4 [MessageBoxA]%ms 0 title message 0;;
+  PUSH _ (SrcI OpSize4 #0);;
+  PUSH _ (SrcI OpSize4 (low 32 title));;
+  PUSH _ (SrcI OpSize4 (low 32 message));;
+  PUSH _ (SrcI OpSize4 #0);;
+  CALLrel _ (JmpTgtRegMem AdSize4 (RegMemM _ _ [OffsetMemSpec AdSize4 (low 32 MessageBoxA)]%ms));;
+(*  call_with stdcall 4 [OffsetMemSpec _ (low 32 MessageBoxA)]%ms 0 title message 0;;*)
   RET 0;
 SECTION DATA
   message:;; dsz "Hello, world";;
@@ -26,5 +32,5 @@ SECTION DATA
 (*=End *)
 
 (*=makeEXE *)
-Compute makeEXE #x"10E30000" "messagebox.exe" mbProg.
+Compute makeEXE #x"0000000010E30000" "messagebox.exe" mbProg.
 (*=End *)
